program_logic/weakestpre.v
@@ -206,6 +206,8 @@ Proof. by apply wp_mask_frame_mono. Qed.
 Global Instance wp_mono' E e :
   Proper (pointwise_relation _ (⊑) ==> (⊑)) (@wp Λ Σ E e).
 Proof. by intros Q Q' ?; apply wp_mono. Qed.
+Lemma wp_strip_pvs E e P Q : P ⊑ wp E e Q → pvs E E P ⊑ wp E e Q.
+Proof. move=>->. by rewrite pvs_wp. Qed.
 Lemma wp_value' E Q e v : to_val e = Some v → Q v ⊑ wp E e Q.
 Proof. intros; rewrite -(of_to_val e v) //; by apply wp_value. Qed.
 Lemma wp_frame_l E e Q R : (R ★ wp E e Q) ⊑ wp E e (λ v, R ★ Q v).
